wip result

Result.v
@@ -8,26 +8,43 @@ Require Import Preorder.
 
 Inductive result (A S : Type) : Type :=
   | returnR : A -> S -> result A S
-  | crashed : result  A S
+  | crashed : result A S
   | exception : S -> result A S.
+  
+Inductive abstract_result (A S : Type) :=
+  | returnRA : A -> S -> abstract_result A S
+  | crashedA : abstract_result A S
+  | exceptionA : S -> abstract_result A S
+  | exceptionOrReturn : A -> S -> abstract_result A S.
 
 Section result_preorder.
 Context {A S: Type} `{PreorderedSet A, PreorderedSet S}.
 
-Inductive result_le : result A S -> result A S -> Prop :=
-  | result_le_crashed : forall r, result_le r (crashed A S)
+Inductive result_le : abstract_result A S -> abstract_result A S -> Prop :=
+  | result_le_crashed : forall r, result_le r (crashedA A S)
   | result_le_exception : forall s1 s2, 
-      preorder s1 s2 -> result_le (exception A S s1) (exception A S s2)
+      preorder s1 s2 -> result_le (exceptionA A S s1) (exceptionA A S s2)
   | result_le_return : forall a1 a2 s1 s2, 
       preorder a1 a2 -> 
       preorder s1 s2 ->
-      result_le (returnR A S a1 s1) (returnR A S a2 s2).
+      result_le (returnRA A S a1 s1) (returnRA A S a2 s2)
+  | result_le_exception_or : forall a st1 st2, 
+      preorder st1 st2 -> 
+      result_le (exceptionA A S st1) (exceptionOrReturn A S a st2)
+  | result_le_return_or : forall a1 a2 s1 s2,
+      preorder s1 s2 ->
+      preorder a1 a2 ->
+      result_le (returnRA A S a1 s1) (exceptionOrReturn A S a2 s2)
+  | result_le_or_or : forall a1 a2 s1 s2,
+      preorder a1 a2 ->
+      preorder s1 s2 ->
+      result_le (exceptionOrReturn A S a1 s1) (exceptionOrReturn A S a2 s2).
+
 
 Lemma result_le_refl :
   Reflexive result_le.
 Proof.
-  unfold Reflexive. destruct x; constructor;
-  apply preorder_refl.
+  unfold Reflexive. destruct x; try constructor; try apply preorder_refl.
 Qed.
 
 Lemma result_le_trans :
@@ -36,14 +53,11 @@ Proof.
   unfold Transitive.
   intros x y z H1 H2.
   inversion H1; inversion H2; subst; 
-  try constructor; try inversion H2; subst. 
-  injection H7 as H9; subst. eapply preorder_trans.
-  apply H3. apply H6.
-  eapply preorder_trans.  apply H3. apply H11.
-  eapply preorder_trans. apply H4. apply H13.
+  try constructor; try inversion H2; subst; auto; eapply preorder_trans;
+  try apply H3; try apply H4; auto.
 Qed.
 
-Global Instance result_preorder : PreorderedSet (result A S) := {
+Global Instance result_preorder : PreorderedSet (abstract_result A S) := {
   preorder := result_le;
   preorder_refl := result_le_refl;
   preorder_trans := result_le_trans;
@@ -53,12 +67,16 @@ End result_preorder.
 Section result_joinable.
 Context {A S : Type} `{Joinable A, Joinable S}.
 
-Definition join_result (r1 r2 : result A S) : result A S :=
+Definition join_result (r1 r2 : abstract_result A S) : abstract_result A S :=
   match r1, r2 with
-  | crashed _ _, _ | _, crashed _ _ => crashed A S
-  | exception _ _ s1, exception _ _ s2 => exception A S (join_op s1 s2)
-  | returnR _ _ a1 s1, returnR _ _ a2 s2 => returnR A S (join_op a1 a2) (join_op s1 s2)
-  | _ , _ => crashed A S
+  | crashedA _ _, _ | _, crashedA _ _ => crashedA A S
+  | exceptionA _ _ s1, exceptionA _ _ s2 => exceptionA A S (join_op s1 s2)
+  | returnRA _ _ a1 s1, returnRA _ _ a2 s2 => returnRA A S (join_op a1 a2) (join_op s1 s2)
+  | exceptionA _ _ s1, returnRA _ _ a2 s2 => exceptionOrReturn A S a2 (join_op s1 s2)
+  | returnRA _ _ a1 s1, exceptionA _ _ s2 => exceptionOrReturn A S a1 (join_op s1 s2)
+  | exceptionOrReturn _ _ a1 s1, exceptionOrReturn _ _ a2 s2 =>
+      exceptionOrReturn A S (join_op a1 a2) (join_op s1 s2)
+  | _ , _ => crashedA A S
   end.
 
 Lemma join_result_upperbound_left :
@@ -67,8 +85,13 @@ Proof.
   intros r1 r2. simpl. destruct r1.
   - destruct r2; simpl; constructor. simpl. 
     apply join_upper_bound_left. apply join_upper_bound_left.
+    apply join_upper_bound_left. apply preorder_refl.
   - simpl. constructor.
   - simpl. destruct r2; simpl; try constructor.
+    apply join_upper_bound_left.
+    apply join_upper_bound_left.
+  - simpl. destruct r2; simpl; try constructor.
+    apply join_upper_bound_left.
     apply join_upper_bound_left.
 Qed.
 
@@ -79,12 +102,18 @@ Proof.
   - destruct r2; simpl; constructor. simpl. 
     apply join_upper_bound_right.
     apply join_upper_bound_right.
+    apply join_upper_bound_right.
   - simpl. constructor.
   - simpl. destruct r2; simpl; constructor.
     apply join_upper_bound_right.
+    apply preorder_refl.
+    apply join_upper_bound_right.
+  - simpl. destruct r2; simpl; try constructor.
+    apply join_upper_bound_right.
+    apply join_upper_bound_right.
 Qed.
 
-Global Instance result_joinable : Joinable (result A S) := {
+Global Instance result_joinable : Joinable (abstract_result A S) := {
   join_op := join_result;
   join_upper_bound_left := join_result_upperbound_left;
   join_upper_bound_right := join_result_upperbound_right;
